src/tools/lifter/bir_lifting_machinesScript.sml
@@ -9,6 +9,7 @@ open bir_exp_liftingTheory
 open bir_temp_varsTheory
 open bir_programTheory
 open bir_program_labelsTheory;
+open bir_interval_expTheory
 
 open arm8Theory arm8_stepTheory
 open m0Theory m0_stepTheory
@@ -460,6 +461,15 @@ val WF_bmr_ms_mem_contains_def = Define `WF_bmr_ms_mem_contains (ba: 'a word, wl
   (LENGTH wl < dimword (:'a)) /\
   (WI_wf (bmr_ms_mem_contains_interval (ba, wl)))`
 
+val WF_bmr_ms_mem_contains_ALT_DEF = store_thm ("WF_bmr_ms_mem_contains_ALT_DEF",
+ ``!(wl:'b word list) (b:'a word).
+   WF_bmr_ms_mem_contains (b,wl) <=>
+   (w2n b + LENGTH wl < dimword (:'a))``,
+
+SIMP_TAC std_ss [WF_bmr_ms_mem_contains_def, WI_wf_def, bmr_ms_mem_contains_interval_def,
+  WI_wf_size, bir_nzcv_expTheory.nzcv_BIR_ADD_C_CARRY_DEF,
+  add_with_carry_def, LET_THM, n2w_w2n, w2n_n2w] >>
+SIMP_TAC (arith_ss++boolSimps.CONJ_ss) []);
 
 
 (**********)
